...

code/Prpu_Benchmark.sml
@@ -1,0 +1,188 @@
+open Prpu
+
+structure Profile = MLton.Profile
+
+val profData = Profile.Data.malloc ()
+
+exception FAILED
+
+fun fail msg = (print (msg ^ "\n"); raise FAILED)
+
+fun 
+  the_fail NONE msg = fail msg
+| the_fail (SOME x) msg = x
+
+val int_of_gi = IntInf.toInt o integer_of_int
+val gi_of_int = Int_of_integer o IntInf.fromInt
+val int_of_gn = IntInf.toInt o integer_of_nat
+val gn_of_int = nat_of_integer o IntInf.fromInt
+
+
+fun readList (infile : string) = let
+  val ins = TextIO.openIn infile
+  fun loop ins =
+   case TextIO.inputLine ins of
+      NONE      => []
+    | SOME line => line :: loop ins
+in
+  let 
+    fun parse_integer s = case Int.fromString s of
+      SOME i => i
+    | NONE => fail ("Expected integer, but got '" ^ s ^"'")  
+
+    val parse_int = gi_of_int o parse_integer
+    val parse_nat = gn_of_int o parse_integer
+
+    val tokenize = String.tokens (fn c => c = #" ")
+    
+    fun parse_edge s = let
+      val l = tokenize s
+    in
+      case l of 
+        [u,v,c] => (parse_nat u, (parse_nat v, parse_int c))
+      | _ => fail ("Expected edge in format 'u v c', but got " ^ s)
+    end
+    
+    fun parse_counts s = let 
+      val l = tokenize s
+    in
+      case l of 
+        [numV,numE] => (parse_integer numV, parse_integer numE)
+      | _ => fail ("Expected counts in format 'numV numE', but got " ^ s)
+    end    
+
+
+    fun parse_graph (counts :: edges) = (parse_counts counts, map parse_edge edges)
+      | parse_graph _ = fail "Empty graph file"
+    
+
+    val lines = (loop ins before TextIO.closeIn ins)
+    val ((numV,numE),edges) = parse_graph lines
+    
+    
+    (*  
+    fun rem_opt i = 
+    case i of
+      NONE   => nat_of_integer (0)
+    | SOME x => nat_of_integer (x) 
+
+    fun rem_opti i = 
+    case i of
+      NONE   => Int_of_integer (0)
+    | SOME x => Int_of_integer (x) 
+    
+    fun line_parse lines = 
+     case lines of
+        []        => []
+      | (l :: ls) => let val toks = ((String.tokens (fn c => c = #" ")) l)
+        in
+          (rem_opt (Int.fromString(hd toks)),
+           (rem_opt (Int.fromString(hd (tl toks))),
+           rem_opti (Int.fromString(hd (tl (tl toks)))))) :: line_parse ls 
+        end 
+    *)      
+  in
+    (numV,edges)
+  end
+end
+
+
+
+
+
+fun the (SOME x) = x
+
+local        
+  fun measure f = let
+    val _ = MLton.GC.collect ();
+    val _ = MLton.GC.unpack ();   
+    val ts = Time.now ()
+    val raw_res = Profile.withData (profData,f)
+    val ts = Time.- (Time.now (), ts) 
+  in (ts,raw_res) end  
+
+  fun iterate n t f = let
+      val _ = print (Int.toString n)
+      val (ts, raw_res) = measure f
+      val t = Time.+ (t,ts)
+      val _ = print ("(" ^ Time.toString ts ^ "s). ")
+    in 
+      if n>1 then 
+        iterate (n-1) t f
+      else  
+        (t,raw_res)
+    end
+  
+in  
+  fun measure n { prepare, run , compres } = let
+    val _ = print ("Netcheck ...");
+    val G = prepare ()  
+    val G = the_fail G "Failed"
+    val _ = print ("Done\n");
+    
+    val _ = print ("Fifo");
+    val (t,res) = iterate n Time.zeroTime (run G)
+    val t = Time.fromNanoseconds (Time.toNanoseconds t div (IntInf.fromInt n))
+    val res = compres res
+    val _ = print ("\n");
+    val _ = print ("@@@time: " ^ IntInf.toString (Time.toMilliseconds t) ^ " ms\n");
+    val _ = print ("@@@max-flow: " ^ res ^ "\n")
+  in () end
+
+end
+
+
+fun fifo_fun s t G = let
+  val s = gn_of_int s
+  val t = gn_of_int t
+in
+  {
+    prepare = fn () => let 
+      val pr = the_fail (fifo_push_relabel_prepare_impl G s t ()) "prepareNet failed"
+    in
+      SOME pr
+    end  ,
+
+    run = fn (N,(am,(c,cf))) => fn () => (N,c,am,fifo_push_relabel_run_impl s t N am cf ()),
+    compres = fn (N,c,am,cf) => let
+        val flow = compute_flow_val_impl s N am cf ()
+      in
+        Int.toString (int_of_gi flow) 
+      end
+  }
+end
+
+
+
+fun main () = let
+  val args = CommandLine.arguments ();
+  
+  fun perform s t G = (
+    measure 1 (fifo_fun s t G);
+    print ("stat_push_c = " ^ Int.toString (!stat.push_c) ^ "\n");
+    print ("stat_relabel_c = " ^ Int.toString (!stat.relabel_c) ^ "\n");
+    print ("stat_gap_c = " ^ Int.toString (!stat.gap_c) ^ "\n");
+    Profile.Data.write(profData,"mlmon.prof.out");
+    Profile.Data.free(profData)
+  )
+  
+in 
+  case args of 
+    [s,t,gname] => let
+      val s = the (Int.fromString s)
+      val t = the (Int.fromString t)
+      val (_,G) = readList gname
+    in  
+      perform s t G
+    end
+  | [gname] => let
+      val (N,G) = readList gname
+      val s = 0
+      val t = N - 1
+    in    
+      perform s t G
+    end
+    | _ => print "Usage: Fifo [<s> <t>] <file-name>\n  If s and t not specified, nodes 0 and |V|-1 are taken."
+end
+
+val _ = if MLton.isMLton then main() else ()
