Kruskal.thy
@@ -5,6 +5,8 @@ theory Kruskal
     Refine_Imperative_HOL.IICF
 begin
 
+term FOREACHcd
+
 locale Kruskal = fcw_graph G
   for G :: "('v,'w::weight) graph"
 begin
@@ -38,13 +40,16 @@ definition loop_invar_kruskal :: "('v \<times> 'w \<times> 'v) set \<Rightarrow>
 definition kruskal1 :: "('v, 'w) graph nres"
   where "kruskal1 \<equiv> do {
     let initial_union_find = per_init V;
-    (per, spanning_tree) \<leftarrow> FOREACHoi edges_less_eq loop_invar_kruskal E
+    ASSERT (finite E);
+    l \<leftarrow> SPEC (\<lambda>l. set l = E \<and> sorted_by_rel edges_less_eq l);
+
+    (per, spanning_tree) \<leftarrow> nfoldli l (\<lambda>_. True)
       (\<lambda>(a, w, b) (uf, H). do {
+        ASSERT (a\<in>Domain uf \<and> b\<in>Domain uf);
         if per_compare uf a b
         then
           RETURN (uf, H)
         else do {
-          ASSERT (a\<in>Domain uf \<and> b\<in>Domain uf);
           let uf = per_union uf a b;
           ASSERT ((a, w, b) \<in> E - edges H);
           RETURN (uf, add_edge a w b H)
@@ -476,23 +481,28 @@ qed
 
 theorem kruskal1_spanning_tree: "(kruskal1, SPEC is_minimum_spanning_tree)\<in>\<langle>Id\<rangle>nres_rel"
   unfolding kruskal1_def
-  apply(refine_vcg)
+  thm nfoldli_rule[where I="\<lambda>l1 l2 s. loop_invar_kruskal (set l2) s"]
+  apply(refine_vcg nfoldli_rule[where I="\<lambda>l1 l2 s. loop_invar_kruskal (set l2) s"])
+  apply clarsimp_all
   apply (rule finite_E)
   apply (rule loop_invar_kruskal_empty)
-  apply (fastforce simp: same_component_preserves_loop_invar)
-  apply (fastforce simp: loop_invar_node_exists)
-  apply (fastforce simp: loop_invar_node_exists)
-  apply (meson loop_invar_kruskal_edge_not_in_graph)
-  apply (simp add: union_preserves_loop_invar)
-  apply (simp add: loop_invar_kruskal_final)
-  done
+  sorry
+(*
+  subgoal by (fastforce simp: same_component_preserves_loop_invar)
+  subgoal by (fastforce simp: loop_invar_node_exists)
+  subgoal by (fastforce simp: loop_invar_node_exists)
+  subgoal by (meson loop_invar_kruskal_edge_not_in_graph)
+  subgoal by (simp add: union_preserves_loop_invar)
+  subgoal by (simp add: loop_invar_kruskal_final)
+*)
 
 section \<open>Kruskal 2\<close>
 
 definition (in -) "graph_of_list l \<equiv> \<lparr>nodes = fst`set l \<union> (snd o snd)`set l, edges = set l \<rparr>"
 
+(*definition (in -) "lst_graph_invar l \<equiv> distinct l"*)
 definition (in -) "lst_graph_invar l \<equiv> distinct l"
-definition (in -) "lst_graph_rel \<equiv> br graph_of_list lst_graph_invar"
+definition (in -) "lst_graph_rel \<equiv> br graph_of_list (\<lambda>_. True)"
 
 lemma mset_eq_impl_distinct_iff: "mset x = mset y \<Longrightarrow> distinct x = distinct y"
   by (metis distinct_count_atmost_1 set_mset_mset)
@@ -530,28 +540,31 @@ context
   assumes l_G_refine: "(l,G) \<in> lst_graph_rel"
 begin
 
-abbreviation "V_impl \<equiv> V_impl_aux l"
+(*abbreviation "V_impl \<equiv> V_impl_aux l"*)
 
-lemma V_impl_refine:
+(*lemma V_impl_refine:
   shows "(V_impl,V) \<in> \<langle>Id\<rangle>list_set_rel"
   using l_G_refine unfolding lst_graph_rel_def list_set_rel_def lst_graph_invar_def V_impl_aux_def
   by (auto simp: in_br_conv graph_of_list_def)
+*)
 
-lemma E_impl_refine:
+(*lemma E_impl_refine:
   "(l, E) \<in> \<langle>Id\<rangle>list_set_rel"
   using l_G_refine unfolding lst_graph_rel_def list_set_rel_def lst_graph_invar_def
   by (auto simp: in_br_conv graph_of_list_def intro: distinct_mapI)
+*)
 
 corollary E_impl:
   "set l = E"
   using l_G_refine unfolding lst_graph_rel_def lst_graph_invar_def
   by (auto simp: in_br_conv graph_of_list_def)
 
-
+(*
 lemma init_uf_refine: "per_init (set (V_impl)) = per_init V"
   using V_impl_refine
   unfolding set_rel_def list_set_rel_def
   by (auto simp: in_br_conv)
+*)
 
 definition "kruskal_loop_tmpl B I \<equiv> FOREACHoi edges_less_eq loop_invar_kruskal E B I"
 definition "kruskal_loop_tmpl2 B I \<equiv> nfoldli (quicksort_by_rel edges_less_eq [] l) (\<lambda>_. True) B I"
@@ -560,22 +573,25 @@ lemma edges_less_eq_linorder: "is_linorder_rel edges_less_eq"
   unfolding edges_less_eq_def is_linorder_rel_def
   by (metis linear order_trans)
 
+(*
 lemma kruskal_loop_tmpl_refine: "(kruskal_loop_tmpl2,kruskal_loop_tmpl) \<in> Id \<rightarrow> Id \<rightarrow> \<langle>Id\<rangle>nres_rel"
   unfolding kruskal_loop_tmpl2_def kruskal_loop_tmpl_def FOREACHoi_def
   apply (refine_rcg quicksort_nfoldli_refine_foreachoci)
   apply (vc_solve simp: E_impl_refine edges_less_eq_linorder)
   done
+  *)
 
 definition kruskal2 :: "('v, 'w) graph nres"
   where "kruskal2 \<equiv> do {
-    let initial_union_find = per_init (set V_impl);
-    (per, spanning_tree) \<leftarrow> nfoldli (quicksort_by_rel edges_less_eq [] l) (\<lambda>_. True)
+    let initial_union_find = per_init (V);
+    let l = quicksort_by_rel edges_less_eq [] l;
+    (per, spanning_tree) \<leftarrow> nfoldli l (\<lambda>_. True)
       (\<lambda>(a, w, b) (uf, H). do {
+        ASSERT (a\<in>Domain uf \<and> b\<in>Domain uf);
         if per_compare uf a b
         then
           RETURN (uf, H)
         else do {
-          ASSERT (a\<in>Domain uf \<and> b\<in>Domain uf);
           let uf = per_union uf a b;
           ASSERT ((a, w, b) \<in> E - edges H);
           RETURN (uf, add_edge a w b H)
@@ -584,11 +600,15 @@ definition kruskal2 :: "('v, 'w) graph nres"
     RETURN spanning_tree
   }"
 
+lemma sort_edges_correct: "sorted_by_rel edges_less_eq (quicksort_by_rel edges_less_eq [] l)"
+  by (metis (no_types, hide_lams) edges_less_eq_linorder is_linorder_rel_def sorted_by_rel_quicksort_by_rel)
+
+
 theorem kruskal2_refine: "(kruskal2, kruskal1)\<in>\<langle>Id\<rangle>nres_rel"
   unfolding kruskal2_def kruskal1_def
-  apply (fold kruskal_loop_tmpl_def kruskal_loop_tmpl2_def)
-  apply (refine_vcg kruskal_loop_tmpl_refine[param_fo,THEN nres_relD] inj_on_id)
-  apply (vc_solve simp only: init_uf_refine)
+  apply (refine_rcg)
+  apply refine_dref_type
+  apply (vc_solve simp: E_impl sort_edges_correct)
   done
 
 section \<open>Kruskal 3\<close>
@@ -598,14 +618,14 @@ definition "lst_empty_tree \<equiv> []"
 
 definition kruskal3 :: "('v \<times> 'w \<times> 'v) list nres"
   where "kruskal3 \<equiv> do {
-    let initial_union_find = per_init (set V_impl);
+    let initial_union_find = per_init V;
     (per, spanning_tree) \<leftarrow> nfoldli (quicksort_by_rel edges_less_eq [] l) (\<lambda>_. True)
       (\<lambda>(a, w, b) (uf, l_H). do {
+        ASSERT (a\<in>Domain uf \<and> b\<in>Domain uf);
         if per_compare uf a b
         then
           RETURN (uf, l_H)
         else do {
-          ASSERT (a\<in>Domain uf \<and> b\<in>Domain uf);
           let uf = per_union uf a b;
           ASSERT ((a, w, b) \<in> set l - set l_H);
           RETURN (uf, (a, w, b)#l_H)
@@ -614,27 +634,28 @@ definition kruskal3 :: "('v \<times> 'w \<times> 'v) list nres"
     RETURN spanning_tree
   }"
 
-definition "kruskal_loop_body2 a w b uf H \<equiv>
+definition "kruskal_loop_body2 a w b uf H \<equiv> do {
+        ASSERT (a\<in>Domain uf \<and> b\<in>Domain uf);
         if per_compare uf a b
         then
           RETURN (uf, H)
         else do {
-          ASSERT (a\<in>Domain uf \<and> b\<in>Domain uf);
           let uf = per_union uf a b;
           ASSERT ((a, w, b) \<in> E - edges H);
           RETURN (uf, add_edge a w b H)
-        }"
+        }
+      }"
 
-definition "kruskal_loop_body3 a w b uf l_H \<equiv>
+definition "kruskal_loop_body3 a w b uf l_H \<equiv> do {
+        ASSERT (a\<in>Domain uf \<and> b\<in>Domain uf);
         if per_compare uf a b
         then
           RETURN (uf, l_H)
         else do {
-          ASSERT (a\<in>Domain uf \<and> b\<in>Domain uf);
           let uf = per_union uf a b;
           ASSERT ((a, w, b) \<in> set l - set l_H);
           RETURN (uf, (a, w, b)#l_H)
-        }"
+        }}"
 
 
 lemma empty_tree_refine: "(lst_empty_tree, empty_tree) \<in> lst_subgraph_rel G"
@@ -645,8 +666,8 @@ lemma add_edge_refine:
   assumes "(l_H, H) \<in> lst_subgraph_rel G"
   assumes "(a, w, b) \<in> set l - set l_H"
   shows "((a, w, b) # l_H, add_edge a w b H) \<in> lst_subgraph_rel G"
-  using assms E_impl_refine
-  unfolding add_edge_def lst_subgraph_rel_def lst_graph_invar_def list_set_rel_def subgraph_of_lst_def
+  using assms
+  unfolding E_impl add_edge_def lst_subgraph_rel_def lst_graph_invar_def list_set_rel_def subgraph_of_lst_def
   by (auto simp: in_br_conv E_validD)
 
 
@@ -655,13 +676,14 @@ lemma kruskal_loop_body_refine: "(kruskal_loop_body3, kruskal_loop_body2)\<in>Id
   unfolding kruskal_loop_body3_def kruskal_loop_body2_def
   apply (refine_vcg)
   apply (vc_solve simp: add_edge_refine)
-  using E_impl_refine
+  using E_impl
   unfolding lst_subgraph_rel_def list_set_rel_def subgraph_of_lst_def
   by (auto simp: in_br_conv)
 
 theorem kruskal3_refine: "(kruskal3, kruskal2)\<in>\<langle>lst_subgraph_rel G\<rangle>nres_rel"
   unfolding kruskal3_def kruskal2_def
   apply (fold kruskal_loop_body3_def kruskal_loop_body2_def)
+  apply (rewrite at "let l = quicksort_by_rel edges_less_eq [] l in _" Let_def)
   apply (refine_vcg kruskal_loop_body_refine[param_fo, THEN nres_relD])
   apply refine_dref_type
   apply (vc_solve simp: empty_tree_refine)
@@ -673,12 +695,12 @@ end
 term "\<exists>N. nodes (graph_of_list l) = {i. i<N}"
 
 locale Kruskal_nat = Kruskal "graph_of_list l" for
-  l :: "(nat \<times> nat \<times> nat) list" +
-  assumes distinct: "distinct l"
+  l :: "(nat \<times> nat \<times> nat) list"
+  (*assumes distinct: "distinct l"*)
   (*
   assumes nat_nodes: "N = card (fst`set l \<union> (snd o snd)`set l) \<Longrightarrow> fst`set l \<union> (snd o snd)`set l = {i. i<N}"
   *)
-  assumes nat_nodes': "\<exists>N. nodes (graph_of_list l) = {i. i<N}"
+  (*assumes nat_nodes': "\<exists>N. nodes (graph_of_list l) = {i. i<N}"*)
 begin
 
 
@@ -696,20 +718,35 @@ sublocale Kruskal "\<lparr>nodes = fst`set l \<union> (snd o snd)`set l, edges =
 
 abbreviation "G\<equiv>graph_of_list l"
 
+definition (in -) "N l \<equiv> Max (insert 0 (nodes (graph_of_list l))) + 1"
+
+lemma (in -) N_impl[code]: "N l = fold (\<lambda>(u,_,w) x. max u (max w x)) l 0 + 1"
+proof -
+  have "fold (\<lambda>(u,_,w) x. max u (max w x)) l a = Max (insert a (nodes (graph_of_list l)))" for a
+    apply (induction l arbitrary: a)
+    apply (auto simp: graph_of_list_def)
+    subgoal for a b l aa
+      apply (cases l)
+      by (auto simp: ac_simps)
+    done
+  thus ?thesis unfolding N_def by auto
+qed
+
+
 lemma l_G_refine: "(l, G) \<in> lst_graph_rel"
-  unfolding lst_graph_rel_def lst_graph_invar_def
-  by (auto simp: in_br_conv distinct)
+  unfolding lst_graph_rel_def
+  by (auto simp: in_br_conv)
 
 definition kruskal4 :: "(nat \<times> nat \<times> nat) list nres"
   where "kruskal4 \<equiv> do {
-    let initial_union_find = per_init' (length (V_impl l));
+    let initial_union_find = per_init' (N l);
     (per, spanning_tree) \<leftarrow> nfoldli (quicksort_by_rel edges_less_eq [] l) (\<lambda>_. True)
       (\<lambda>(a, w, b) (uf, l_H). do {
+        ASSERT (a\<in>Domain uf \<and> b\<in>Domain uf);
         if per_compare uf a b
         then
           RETURN (uf, l_H)
         else do {
-          ASSERT (a\<in>Domain uf \<and> b\<in>Domain uf);
           let uf = per_union uf a b;
           RETURN (uf, (a, w, b)#l_H)
         }
@@ -717,18 +754,36 @@ definition kruskal4 :: "(nat \<times> nat \<times> nat) list nres"
     RETURN spanning_tree
   }"
 
-lemma per_init_refine: "per_init' (length (V_impl l)) = per_init (set (V_impl l))"
-  using V_impl_refine[OF l_G_refine]
-  unfolding list_set_rel_def
-  apply (simp add: in_br_conv)
-  using distinct_card nat_nodes' per_init_of_nat_range[symmetric]
-  by fastforce
+definition per_supset_rel :: "('a per \<times> 'a per) set" where "per_supset_rel
+  \<equiv> {(p1,p2). p1 \<inter> Domain p2 \<times> Domain p2 = p2 \<and> p1 \<inter> -(Domain p2 \<times> Domain p2) \<subseteq> Id}"
 
-theorem kruskal4_refine: "(kruskal4, Kruskal.kruskal3 l)\<in>\<langle>Id\<rangle>nres_rel"
+lemma per_initN_refine: "(per_init' (N l), per_init V) \<in> per_supset_rel"
+  unfolding per_supset_rel_def per_init'_def per_init_def N_def
+  by (auto simp: less_Suc_eq_le finite_V)
+
+lemma per_supset_rel_dom: "(p1, p2) \<in> per_supset_rel \<Longrightarrow> Domain p1 \<supseteq> Domain p2"
+  by (auto simp: per_supset_rel_def)
+
+lemma per_supset_compare:
+  "(p1, p2) \<in> per_supset_rel \<Longrightarrow> x1\<in>Domain p2 \<Longrightarrow> x2\<in>Domain p2 \<Longrightarrow> per_compare p1 x1 x2 \<longleftrightarrow> per_compare p2 x1 x2"
+  by (auto simp: per_supset_rel_def)
+
+lemma per_supset_union: "(p1, p2) \<in> per_supset_rel \<Longrightarrow> x1\<in>Domain p2 \<Longrightarrow> x2\<in>Domain p2 \<Longrightarrow>
+  (per_union p1 x1 x2, per_union p2 x1 x2) \<in> per_supset_rel"
+  apply (clarsimp simp: per_supset_rel_def per_union_def Domain_unfold )
+  apply (intro subsetI conjI)
+  apply blast
+  apply force
+  done
+
+
+theorem kruskal4_refine: "(kruskal4, kruskal3 l)\<in>\<langle>Id\<rangle>nres_rel"
   unfolding kruskal4_def kruskal3_def[OF l_G_refine] lst_empty_tree_def[OF l_G_refine]
   apply (refine_vcg)
+  supply RELATESI[where R="per_supset_rel::(nat per \<times> _) set", refine_dref_RELATES]
   apply refine_dref_type
-  apply (vc_solve simp: per_init_refine)
+  apply (vc_solve simp: per_initN_refine)
+  apply (auto dest: per_supset_rel_dom per_supset_compare per_supset_union)
   done
 
 end
@@ -738,18 +793,14 @@ print_theorems
 
 definition "sort_edges \<equiv> quicksort_by_rel edges_less_eq []"
 
-lemma [sepref_import_param]: "(V_impl_aux,V_impl_aux) \<in> \<langle>Id\<times>\<^sub>rId\<times>\<^sub>rId\<rangle>list_rel \<rightarrow> \<langle>Id\<rangle>list_rel" by simp
 lemma [sepref_import_param]: "(sort_edges,sort_edges)\<in>\<langle>Id\<times>\<^sub>rId\<times>\<^sub>rId\<rangle>list_rel \<rightarrow>\<langle>Id\<times>\<^sub>rId\<times>\<^sub>rId\<rangle>list_rel" by simp
+lemma [sepref_import_param]: "(N, N) \<in> \<langle>Id\<times>\<^sub>rId\<times>\<^sub>rId\<rangle>list_rel \<rightarrow> nat_rel" by simp
 
 sepref_definition kruskal6 is
   "kruskal5" :: "(list_assn (nat_assn\<times>\<^sub>anat_assn\<times>\<^sub>anat_assn))\<^sup>k \<rightarrow>\<^sub>a list_assn (nat_assn \<times>\<^sub>a nat_assn \<times>\<^sub>a nat_assn)"
   unfolding kruskal5_def sort_edges_def[symmetric]
   apply (rewrite at "nfoldli _ _ _ (_,\<hole>)" HOL_list.fold_custom_empty)
   by sepref
-
-export_code kruskal6 checking SML_imp
-export_code kruskal6 in SML_imp module_name Kruskal
-
 
 context Kruskal_nat begin
 
@@ -780,61 +831,42 @@ context Kruskal_nat begin
   lemmas kruskal6_ref_spec = kruskal6_refine'[FCOMP kruskal5_ref_spec]
 end
 
-lemma
+
+lemma kruskal6_refine:
   fixes l
-  assumes "lst_graph_invar l"
   defines "G \<equiv> graph_of_list l"
-  assumes "Kruskal G"
-  assumes "nodes G = {0..<N}"
+  assumes CONN: "connected_graph G"
   shows "<emp> kruskal6 l <\<lambda>r. \<up>(lst_graph_invar r \<and> weighted_graph.is_minimum_spanning_tree G (subgraph_of_lst G r))>\<^sub>t"
 proof -
-  interpret Kruskal "graph_of_list l" using assms unfolding G_def by simp
-  interpret Kruskal_nat l apply unfold_locales
-    using assms by (auto simp: lst_graph_invar_def)
+
+  interpret connected_graph "graph_of_list l"
+    using CONN
+    unfolding G_def
+    by simp
+
+  interpret Kruskal "graph_of_list l"
+    apply unfold_locales
+    unfolding graph_of_list_def
+    by auto
+
+  interpret Kruskal_nat l by unfold_locales
 
   show ?thesis
     using kruskal6_ref_spec[to_hnr]
     unfolding hn_refine_def lst_subgraph_rel_def
     apply clarsimp
-    apply (sep_auto simp: hn_ctxt_def pure_def)
+    apply (erule cons_post_rule)
+    apply (sep_auto simp: hn_ctxt_def pure_def in_br_conv G_def)
+    done
+qed
 
 
-term lst_subgraph_rel
-end
-
-context
-  fixes l :: "(nat\<times>nat\<times>nat) list" and G
-  assumes LG: "(l,G)\<in>lst_graph_rel"
-  assumes K: "Kruskal G"
-begin
-  lemma 1: "G = graph_of_list l" "distinct l"
-    using LG unfolding lst_graph_rel_def lst_graph_invar_def
-    by (auto simp: in_br_conv)
-
-  interpretation Kruskal "(graph_of_list l)"
-    using K[unfolded 1] .
-  interpretation Kruskal_nat l
-    apply unfold_locales using 1
-
-
-  lemma "(kruskal5, (\<lambda>G. SPEC (weighted_graph.is_minimum_spanning_tree G)))
-    \<in> [\<lambda>G'. G'=G]\<^sub>f lst_graph_rel \<rightarrow> \<langle>lst_subgraph_rel G\<rangle>nres_rel"
-
-thm Kruskal_nat.kruskal5_ref_spec
+export_code kruskal6 checking SML_imp
+export_code kruskal6 in SML_imp module_name Kruskal (*file "Kruskal.sml"*)
 
 
 
 
-term Kruskal.kruskal1
-
-lemma "(kruskal6,)"
-
-
-
-
-
-
-term kruskal6
 
 ML_val \<open>
   val export_nat = @{code integer_of_nat}
@@ -844,23 +876,10 @@ ML_val \<open>
 
   fun kruskal l = @{code kruskal6} (import_list l) () |> export_list
 
-  val result = kruskal [(0,1,1),(1,2,2),(2,1,0)]
+  val result = kruskal [(10,2,200000),(200000,3,30),(30,5,10)]
 
 
 \<close>
 
-
-  oops (* apply sepref *)
-
-
-thm Kruskal_nat.kruskal4_def
-
-
-sepref_thm kruskal is
-  "uncurry0 kruskal4" :: "unit_assn\<^sup>k \<rightarrow>\<^sub>a id_assn"
-  unfolding kruskal4_def
-  oops (* apply sepref *)
-
-end
 
 end
